@prefix : <https://schema.org/> .
@prefix rdf: <http://www.w3.org/1999/02/22-rdf-syntax-ns#> .
@prefix rdfs: <http://www.w3.org/2000/01/rdf-schema#> .


:MediaEnumeration a rdfs:Class ;
rdfs:label "MediaEnumeration" ;
:isPartOf <https://pending.schema.org> ;
:source <https://github.com/schemaorg/schemaorg/issues/3392> ;
rdfs:comment """MediaEnumeration enumerations are lists of codes, labels etc. useful for describing media objects. They may be reflections of externally developed lists, or created at schema.org, or a combination.""" ;
rdfs:subClassOf :Enumeration .

:IPTCDigitalSourceEnumeration a rdfs:Class ;
rdfs:label "IPTCDigitalSourceEnumeration" ;
:isPartOf <https://pending.schema.org> ;
:source <https://github.com/schemaorg/schemaorg/issues/3392> ;
rdfs:comment """<a href="https://www.iptc.org/">IPTC</a> "Digital Source" codes for use with the [[digitalSourceType]] property, providing information about the source for a digital media object. 
In general these codes are not declared here to be mutually exclusive, although some combinations would be contradictory if applied simultaneously, or might be considered mutually incompatible by upstream maintainers of the definitions.
 See the IPTC <a href="https://www.iptc.org/std/photometadata/documentation/userguide/">documentation</a> for <a href="https://cv.iptc.org/newscodes/digitalsourcetype/">detailed definitions</a> of all terms.""" ;
rdfs:subClassOf :MediaEnumeration .

:digitalSourceType a rdf:Property ;
    rdfs:label "digitalSourceType" ;
    :domainIncludes :CreativeWork ;
    :isPartOf <https://pending.schema.org> ;
    :rangeIncludes :IPTCDigitalSourceEnumeration ;
    :source <https://github.com/schemaorg/schemaorg/issues/3392> ;
    rdfs:comment """Indicates an IPTCDigitalSourceEnumeration code indicating the nature of the digital source(s) for some [[CreativeWork]].""" .


#TODO:
#DigitalCaptureDigitalSource
#NegativeFilmDigitalSource
#PositiveFilmDigitalSource
#PrintDigitalSource
#MinorHumanEditsDigitalSource
#CompositeCaptureDigitalSource
#AlgorithmicallyEnhancedDigitalSource
#DataDrivenMediaDigitalSource
#DigitalArtDigitalSource
#VirtualRecordingDigitalSource
#TrainedAlgorithmicMediaDigitalSource
#CompositeSyntheticDigitalSource
#CompositeWithTrainedAlgorithmicMediaDigitalSource
#AlgorithmicMediaDigitalSource

:DigitalCaptureDigitalSource a :IPTCDigitalSourceEnumeration ;
    rdfs:label "DigitalCaptureDigitalSource" ;
    :isPartOf <https://pending.schema.org> ;
    :source <https://github.com/schemaorg/schemaorg/issues/3392> ;
    rdfs:comment  """Content coded 'as digital capture' using the IPTC digital source type vocabulary.""" .

